commit

AP/System/Symmetry/Defs.lean
@@ -10,155 +10,81 @@ structure Symmetry (sys : System S T) : Type u extends Symmetry.Raw sys where
 
 namespace Symmetry
 
-variable {sym sym₁ sym₂ sym₃ : Symmetry sys}
+variable {sym sym₁ sym₂ sym₃ : sys.Symmetry}
 
 @[ext]
 theorem ext (h : sym₁.toRaw = sym₂.toRaw) : sym₁ = sym₂ := by
   cases sym₁; cases sym₂; simp_all
 
-def one : Symmetry sys :=
+def one : sys.Symmetry :=
   ⟨Raw.one, inferInstance⟩
 
-instance : Inhabited (Symmetry sys) := ⟨one⟩
-theorem default_eq : (default : Symmetry sys) = one := rfl
+instance : One sys.Symmetry := ⟨one⟩
+theorem one_def : (1 : sys.Symmetry) = 1 := rfl
+
+instance : Inhabited sys.Symmetry := ⟨1⟩
+theorem default_eq : (default : sys.Symmetry) = 1 := rfl
 
 instance : sym.toRaw.WF := sym.wf
 
-theorem tr_fs {s t} [hs : sys.WF s] :
-sys.tr (sym.fs s) t = (sys.tr s (sym.ft' t)).map sym.fs := Raw.tr_fs
+theorem tr_fs {s t} : sys.tr (sym.fs s) t = (sys.tr s (sym.ft' t)).map sym.fs := Raw.tr_fs
+theorem tr_fs' {s t} : sys.tr (sym.fs' s) t = (sys.tr s (sym.ft t)).map sym.fs' := Raw.tr_fs'
+theorem tr_ft {s t} : sys.tr s (sym.ft t) = (sys.tr (sym.fs' s) t).map sym.fs := Raw.tr_ft
+theorem tr_ft' {s t} : sys.tr s (sym.ft' t) = (sys.tr (sym.fs s) t).map sym.fs' := Raw.tr_ft'
 
-theorem tr_fs' {s t} [hs : sys.WF s] :
-sys.tr (sym.fs' s) t = (sys.tr s (sym.ft t)).map sym.fs' := Raw.tr_fs'
+theorem validTr_fs_of {s t} (h : sys.validTr s (sym.ft' t)) :
+sys.validTr (sym.fs s) t := Raw.validTr_fs_of h
 
-theorem tr_ft {s t} [hs : sys.WF s] :
-sys.tr s (sym.ft t) = (sys.tr (sym.fs' s) t).map sym.fs := Raw.tr_ft
+theorem validTr_fs'_of {s t} (h : sys.validTr s (sym.ft t)) :
+sys.validTr (sym.fs' s) t := Raw.validTr_fs'_of h
 
-theorem tr_ft' {s t} [hs : sys.WF s] :
-sys.tr s (sym.ft' t) = (sys.tr (sym.fs s) t).map sym.fs' := Raw.tr_ft'
+theorem validTr_ft_of {s t} (h : sys.validTr (sym.fs' s) t) :
+sys.validTr s (sym.ft t) := Raw.validTr_ft_of h
 
-theorem validTr_fs_of {s t} [hs : sys.WF s]
-(h : sys.validTr s (sym.ft' t)) : sys.validTr (sym.fs s) t := Raw.validTr_fs_of h
+theorem validTr_ft'_of {s t} (h : sys.validTr (sym.fs s) t) :
+sys.validTr s (sym.ft' t) := Raw.validTr_ft'_of h
 
-theorem validTr_fs'_of {s t} [hs : sys.WF s]
-(h : sys.validTr s (sym.ft t)) : sys.validTr (sym.fs' s) t := Raw.validTr_fs'_of h
+theorem validTr_fs {s t} : sys.validTr (sym.fs s) t ↔
+sys.validTr s (sym.ft' t) := Raw.validTr_fs
 
-theorem validTr_ft_of {s t} [hs : sys.WF s]
-(h : sys.validTr (sym.fs' s) t) : sys.validTr s (sym.ft t) := Raw.validTr_ft_of h
+theorem validTr_fs' {s t} : sys.validTr (sym.fs' s) t ↔
+sys.validTr s (sym.ft t) := Raw.validTr_fs'
 
-theorem validTr_ft'_of {s t} [hs : sys.WF s]
-(h : sys.validTr (sym.fs s) t) : sys.validTr s (sym.ft' t) := Raw.validTr_ft'_of h
+theorem validTr_ft {s t} : sys.validTr s (sym.ft t) ↔
+sys.validTr (sym.fs' s) t := Raw.validTr_ft
 
-theorem validTr_fs {s t} [hs : sys.WF s] :
-sys.validTr (sym.fs s) t ↔ sys.validTr s (sym.ft' t) := Raw.validTr_fs
+theorem validTr_ft' {s t} : sys.validTr s (sym.ft' t) ↔
+sys.validTr (sym.fs s) t := Raw.validTr_ft'
 
-theorem validTr_fs' {s t} [hs : sys.WF s] :
-sys.validTr (sym.fs' s) t ↔ sys.validTr s (sym.ft t) := Raw.validTr_fs'
-
-theorem validTr_ft {s t} [hs : sys.WF s] :
-sys.validTr s (sym.ft t) ↔ sys.validTr (sym.fs' s) t := Raw.validTr_ft
-
-theorem validTr_ft' {s t} [hs : sys.WF s] :
-sys.validTr s (sym.ft' t) ↔ sys.validTr (sym.fs s) t :=
-  ⟨validTr_fs_of, validTr_ft'_of⟩
-
-def simFn (sym : Symmetry sys) (f : S → T) (s : S) : T :=
+def simFn (sym : sys.Symmetry) (f : S → T) (s : S) : T :=
   sym.toRaw.simFn f s
 
 instance {f} [hf : sys.SimFn f] : sys.SimFn (sym.simFn f) := by
   unfold simFn; infer_instance
 
-def inv (sym : Symmetry sys) : Symmetry sys :=
+def inv (sym : sys.Symmetry) : sys.Symmetry :=
   ⟨sym.toRaw.inv, inferInstance⟩
 
-@[simp]
-theorem inv_inv : sym.inv.inv = sym := ext Raw.inv_inv
+instance : Inv sys.Symmetry := ⟨inv⟩
+theorem inv_def : sym⁻¹ = sym.inv := rfl
 
-def mul (sym₁ sym₂ : Symmetry sys) : Symmetry sys :=
+@[simp]
+theorem inv_inv : sym⁻¹⁻¹ = sym := ext Raw.inv_inv
+
+def mul (sym₁ sym₂ : sys.Symmetry) : sys.Symmetry :=
   ⟨sym₁.toRaw.mul sym₂.toRaw, inferInstance⟩
 
-def npow (n : ℕ) (sym : Symmetry sys) : Symmetry sys :=
+instance : Mul sys.Symmetry := ⟨mul⟩
+theorem mul_def : sym₁ * sym₂ = sym₁.mul sym₂ := rfl
+
+def div (sym₁ sym₂ : sys.Symmetry) : sys.Symmetry :=
+  ⟨sym₁.toRaw.div sym₂.toRaw, inferInstance⟩
+
+instance : Div sys.Symmetry := ⟨div⟩
+theorem div_def : sym₁ / sym₂ = sym₁.div sym₂ := rfl
+
+def npow (n : ℕ) (sym : sys.Symmetry) : sys.Symmetry :=
   ⟨sym.toRaw.npow n, inferInstance⟩
 
-def zpow (z : ℤ) (sym : Symmetry sys) : Symmetry sys :=
+def zpow (z : ℤ) (sym : sys.Symmetry) : sys.Symmetry :=
   ⟨sym.toRaw.zpow z, inferInstance⟩
-
-def Equiv (sym₁ sym₂ : Symmetry sys) : Prop :=
-  sym₁.toRaw.Equiv sym₂.toRaw
-
-@[simp, refl]
-theorem Equiv.refl : sym.Equiv sym := Raw.Equiv.refl
-
-@[symm]
-theorem Equiv.symm (h : sym₁.Equiv sym₂) : sym₂.Equiv sym₁ :=
-  Raw.Equiv.symm h
-
-@[trans]
-theorem Equiv.trans (h₁ : sym₁.Equiv sym₂) (h₂ : sym₂.Equiv sym₃) : sym₁.Equiv sym₃ :=
-  Raw.Equiv.trans h₁ h₂
-
-theorem Equiv.iseqv : Equivalence # Equiv (sys := sys) where
-  refl := λ _ => refl
-  symm := symm
-  trans := trans
-
-instance setoid : Setoid (Symmetry sys) where
-  r := Equiv
-  iseqv := Equiv.iseqv
-
-#check 0 #exit
-
-instance : Monoid sys.Symmetry where
-  one_mul := λ _ => rfl
-  mul_one := λ _ => rfl
-  mul_assoc := λ _ _ _ => rfl
-  npow := npow
-  npow_succ := by intros; simp_rw [npow, Function.iterate_succ']; simp
-
-protected theorem inv_one : (1 : sys.Symmetry)⁻¹ = 1 := rfl
-protected theorem mul_inv_rev : (sym₁ * sym₂)⁻¹ = sym₂⁻¹ * sym₁⁻¹ := rfl
-
-#check 0 #exit
-
-protected theorem inv_mul_cancel : sym * sym⁻¹ = 1 := by
-  ext
-  · nm s
-    simp [inv_def, mul_def, one_def, inv, mul, one]
-    simp
-
-#check 0 #exit
-
-instance : Group sys.Symmetry where
-  inv_mul_cancel := by
-
-#check 0 #exit
-
-protected theorem inv_eq_of_mul (h : sym₁ * sym₂ = 1) : sym₁⁻¹ = sym₂ := by
-  apply congrArg (· * sym₂⁻¹) at h
-  simp [mul_assoc] at h
-
-#check 0 #exit
-
-theorem inv_npow {n} : sym⁻¹ ^ n = (sym ^ n)⁻¹ := by
-  induction n; rfl; nm n ih; simp [pow_succ]
-  rw [ih]; clear ih; induction n; rfl; nm n ih
-  simp [pow_succ, Symmetry.mul_inv_rev]; rw [mul_assoc, ih]
-
-instance : DivInvMonoid sys.Symmetry where
-  zpow := zpow
-  zpow_succ' := Monoid.npow_succ
-  zpow_neg' := λ _ _ => inv_npow
-
-instance : DivisionMonoid sys.Symmetry where
-  inv_inv := λ _ => Symmetry.inv_inv
-  mul_inv_rev := λ _ _ => Symmetry.mul_inv_rev
-  inv_eq_of_mul := by
-  -- inv_mul := by
-  --   sorry
-
-#check 0 #exit
-
--- instance : InvOneClass sys.Symmetry where
---   inv_one := Symmetry.inv_one
-
-example : sym ^ (-1 : ℤ) = sym⁻¹ := by
-  rw [zpow_neg]
