AP/System/Symmetry/Raw.lean
@@ -14,11 +14,39 @@ structure Raw (sys : System S T) : Type u where
 
 namespace Raw
 
+section func
+
+structure Inverse {α β : Type*} (f : α → β) (g : β → α) : Prop where
+  fg : ∀ {x}, f (g x) = x
+  gf : ∀ {x}, g (f x) = x
+
+@[simp]
+theorem inverse_id {α : Type*} : Inverse (@id α) id := by
+  constructor <;> simp
+
+namespace Inverse
+
+variable {α β : Type*} {f : α → β} {g : β → α}
+variable {H : Inverse f g}
+include H
+
+@[symm]
+theorem symm : Inverse g f := ⟨H.2, H.1⟩
+
+-- #check 0 #exit
+
+end Inverse
+end func
+
 class WF (sym : Raw sys) : Prop where
-  h_fs : StrictBijectiveOn sys.WF sys.WF sym.fs sym.fs'
-  h_ft : StrictBijectiveOn sys.WFTrans sys.WFTrans sym.ft sym.ft'
-  tr_eq : ∀ {s t} [sys.WF s], sys.tr s t = (sys.tr (sym.fs s) (sym.ft t)).map sym.fs'
-  tr_eq' : ∀ {s t} [sys.WF s], sys.tr s t = (sys.tr (sym.fs' s) (sym.ft' t)).map sym.fs
+  h_fs : ∀ {s}, sys.WF (sym.fs s) ↔ sys.WF s
+  h_fs' : ∀ {s}, sys.WF (sym.fs' s) ↔ sys.WF s
+  h_ft : ∀ {t}, sys.WFTrans (sym.ft t) ↔ sys.WFTrans t
+  h_ft' : ∀ {t}, sys.WFTrans (sym.ft' t) ↔ sys.WFTrans t
+  fs_fs' : Inverse sym.fs sym.fs'
+  ft_ft' : Inverse sym.ft sym.ft'
+  tr_eq : ∀ {s t}, sys.tr s t = (sys.tr (sym.fs s) (sym.ft t)).map sym.fs'
+  tr_eq' : ∀ {s t}, sys.tr s t = (sys.tr (sym.fs' s) (sym.ft' t)).map sym.fs
 
 def one : Raw sys where
   fs := id
@@ -45,6 +73,9 @@ def mul (sym₁ sym₂ : Raw sys) : Raw sys where
   ft := sym₁.ft ∘ sym₂.ft
   ft' := sym₂.ft' ∘ sym₁.ft'
 
+def div (sym₁ sym₂ : Raw sys) : Raw sys :=
+  sym₁.mul sym₂.inv
+
 def npow (n : ℕ) (sym : Raw sys) : Raw sys :=
   (·.mul sym)^[n] one
 
@@ -58,103 +89,72 @@ def zpow (z : ℤ) (sym : Raw sys) : Raw sys :=
 variable {sym sym₁ sym₂ sym₃ : Raw sys}
 variable [wf : sym.WF] [wf₁ : sym₁.WF] [wf₂ : sym₂.WF] [wf₃ : sym₃.WF]
 
-instance {s} [hs : sys.WF s] : sys.WF (sym.fs s) :=
-  wf.h_fs.cnd_right hs
+@[simp] theorem wf_fs_iff {s} : sys.WF (sym.fs s) ↔ sys.WF s := by rw [wf.h_fs]
+@[simp] theorem wf_fs'_iff {s} : sys.WF (sym.fs' s) ↔ sys.WF s := by rw [wf.h_fs']
+@[simp] theorem wf_ft_iff {t} : sys.WFTrans (sym.ft t) ↔ sys.WFTrans t := by rw [wf.h_ft]
+@[simp] theorem wf_ft'_iff {t} : sys.WFTrans (sym.ft' t) ↔ sys.WFTrans t := by rw [wf.h_ft']
 
-instance {s} [hs : sys.WF s] : sys.WF (sym.fs' s) :=
-  wf.h_fs.cnd_left hs
+instance {s} [hs : sys.WF s] : sys.WF (sym.fs s) := by simpa
+instance {s} [hs : sys.WF s] : sys.WF (sym.fs' s) := by simpa
+instance {t} [ht : sys.WFTrans t] : sys.WFTrans (sym.ft t) := by simpa
+instance {t} [ht : sys.WFTrans t] : sys.WFTrans (sym.ft' t) := by simpa
 
-instance {t} [ht : sys.WFTrans t] : sys.WFTrans (sym.ft t) :=
-  wf.h_ft.cnd_right ht
+@[simp] theorem fs_fs' {s} : sym.fs (sym.fs' s) = s := wf.fs_fs'.fg
+@[simp] theorem fs'_fs {s} : sym.fs' (sym.fs s) = s := wf.fs_fs'.gf
+@[simp] theorem ft_ft' {s} : sym.ft (sym.ft' s) = s := wf.ft_ft'.fg
+@[simp] theorem ft'_ft {s} : sym.ft' (sym.ft s) = s := wf.ft_ft'.gf
 
-instance {t} [ht : sys.WFTrans t] : sys.WFTrans (sym.ft' t) :=
-  wf.h_ft.cnd_left ht
-
-include wf
-
-@[simp]
-theorem fs'_fs {s} [hs : sys.WF s] : sym.fs' (sym.fs s) = s :=
-  wf.h_fs.cancel_left hs
-
-@[simp]
-theorem fs_fs' {s} [hs : sys.WF s] : sym.fs (sym.fs' s) = s :=
-  wf.h_fs.cancel_right hs
-
-@[simp]
-theorem ft'_ft {t} [ht : sys.WFTrans t] : sym.ft' (sym.ft t) = t :=
-  wf.h_ft.cancel_left ht
-
-@[simp]
-theorem ft_ft' {t} [ht : sys.WFTrans t] : sym.ft (sym.ft' t) = t :=
-  wf.h_ft.cancel_right ht
-
-theorem tr_fs {s t} [hs : sys.WF s] :
-sys.tr (sym.fs s) t = (sys.tr s (sym.ft' t)).map sym.fs := by
+theorem tr_fs {s t} : sys.tr (sym.fs s) t = (sys.tr s (sym.ft' t)).map sym.fs := by
   nth_rw 1 [wf.tr_eq']; ext s'; simp
 
-theorem tr_fs' {s t} [hs : sys.WF s] :
-sys.tr (sym.fs' s) t = (sys.tr s (sym.ft t)).map sym.fs' := by
+theorem tr_fs' {s t} : sys.tr (sym.fs' s) t = (sys.tr s (sym.ft t)).map sym.fs' := by
   nth_rw 1 [wf.tr_eq]; ext s'; simp
 
-theorem tr_ft {s t} [hs : sys.WF s] :
-sys.tr s (sym.ft t) = (sys.tr (sym.fs' s) t).map sym.fs := by
-  nth_rw 2 [wf.tr_eq]; ext s'; simp; constructor
-  · intro h; use s'; have hs' := wf_of_tr h; simpa
-  · rintro ⟨s₁, h₁, h₂⟩; have hs₁ := wf_of_tr h₁; simp at h₂; simpa [←h₂]
+theorem tr_ft {s t} : sys.tr s (sym.ft t) = (sys.tr (sym.fs' s) t).map sym.fs := by
+  nth_rw 2 [wf.tr_eq]; ext s'; simp
 
-theorem tr_ft' {s t} [hs : sys.WF s] :
-sys.tr s (sym.ft' t) = (sys.tr (sym.fs s) t).map sym.fs' := by
-  nth_rw 2 [wf.tr_eq']; ext s'; simp; constructor
-  · intro h; use s', h; have h₁ := wf_of_tr h; simp
-  · rintro ⟨s₁, h₁, h₂⟩; have h₃ := wf_of_tr h₁; simp at h₂; simpa [←h₂]
+theorem tr_ft' {s t} : sys.tr s (sym.ft' t) = (sys.tr (sym.fs s) t).map sym.fs' := by
+  nth_rw 2 [wf.tr_eq']; ext s'; simp
 
-theorem validTr_fs_of {s t} [hs : sys.WF s]
+theorem validTr_fs_of {s t}
 (h : sys.validTr s (sym.ft' t)) : sys.validTr (sym.fs s) t := by
   obtain ⟨s', h⟩ := h; simp [tr_ft'] at h; obtain ⟨s', h, rfl⟩ := h; use s'
 
-theorem validTr_fs'_of {s t} [hs : sys.WF s]
+theorem validTr_fs'_of {s t}
 (h : sys.validTr s (sym.ft t)) : sys.validTr (sym.fs' s) t := by
   obtain ⟨s', h⟩ := h; simp [tr_ft] at h; obtain ⟨s', h, rfl⟩ := h; use s'
 
-theorem validTr_ft_of {s t} [hs : sys.WF s]
+theorem validTr_ft_of {s t}
 (h : sys.validTr (sym.fs' s) t) : sys.validTr s (sym.ft t) := by
   obtain ⟨s', h⟩ := h; simp [tr_fs'] at h; obtain ⟨s', h, rfl⟩ := h; use s'
 
-theorem validTr_ft'_of {s t} [hs : sys.WF s]
+theorem validTr_ft'_of {s t}
 (h : sys.validTr (sym.fs s) t) : sys.validTr s (sym.ft' t) := by
   obtain ⟨s', h⟩ := h; simp [tr_fs] at h; obtain ⟨s', h, rfl⟩ := h; use s'
 
-theorem validTr_fs {s t} [hs : sys.WF s] :
-sys.validTr (sym.fs s) t ↔ sys.validTr s (sym.ft' t) :=
+theorem validTr_fs {s t} : sys.validTr (sym.fs s) t ↔ sys.validTr s (sym.ft' t) :=
   ⟨validTr_ft'_of, validTr_fs_of⟩
 
-theorem validTr_fs' {s t} [hs : sys.WF s] :
-sys.validTr (sym.fs' s) t ↔ sys.validTr s (sym.ft t) :=
+theorem validTr_fs' {s t} : sys.validTr (sym.fs' s) t ↔ sys.validTr s (sym.ft t) :=
   ⟨validTr_ft_of, validTr_fs'_of⟩
 
-theorem validTr_ft {s t} [hs : sys.WF s] :
-sys.validTr s (sym.ft t) ↔ sys.validTr (sym.fs' s) t :=
+theorem validTr_ft {s t} : sys.validTr s (sym.ft t) ↔ sys.validTr (sym.fs' s) t :=
   ⟨validTr_fs'_of, validTr_ft_of⟩
 
-theorem validTr_ft' {s t} [hs : sys.WF s] :
-sys.validTr s (sym.ft' t) ↔ sys.validTr (sym.fs s) t :=
+theorem validTr_ft' {s t} : sys.validTr s (sym.ft' t) ↔ sys.validTr (sym.fs s) t :=
   ⟨validTr_fs_of, validTr_ft'_of⟩
 
 @[simp]
-theorem hasTr_fs {s} [hs : sys.WF s] :
-sys.hasTr (sym.fs s) ↔ sys.hasTr s := by
+theorem hasTr_fs {s} : sys.hasTr (sym.fs s) ↔ sys.hasTr s := by
   constructor <;> rintro ⟨t, h⟩
   · use sym.ft' t; simpa [validTr_ft']
   · use sym.ft t; simpa [validTr_ft]
 
 @[simp]
-theorem hasTr_fs' {s} [hs : sys.WF s] :
-sys.hasTr (sym.fs' s) ↔ sys.hasTr s := by
+theorem hasTr_fs' {s} : sys.hasTr (sym.fs' s) ↔ sys.hasTr s := by
   constructor <;> rintro ⟨t, h⟩
   · use sym.ft t; simpa [validTr_ft]
   · use sym.ft' t; simpa [validTr_ft']
-
-omit wf
 
 instance : (Raw.one : Raw sys).WF := by
   unfold Raw.one; constructor <;> simp
@@ -163,88 +163,53 @@ instance {f} [hf : sys.SimFn f] : sys.SimFn (sym.simFn f) := by
   rw [sys.simFn_def]; intro s hs h; simp; apply hf.1 at h; apply validTr_ft_of
   have h₁ : sys.hasTr (sym.fs' s); simp; exact ⟨_, h⟩; exact hf.1 h₁
 
-include wf₁ in
-instance [wf : sym.WF] : sym.inv.WF where
-  h_fs := wf.h_fs.symm
-  h_ft := wf.h_ft.symm
+instance : sym.inv.WF where
+  h_fs := wf.h_fs'
+  h_fs' := wf.h_fs
+  h_ft := wf.h_ft'
+  h_ft' := wf.h_ft
+  fs_fs' := wf.fs_fs'.symm
+  ft_ft' := wf.ft_ft'.symm
   tr_eq := wf.tr_eq'
   tr_eq' := wf.tr_eq
 
-@[simp]
+omit wf in @[simp]
 theorem inv_inv : sym.inv.inv = sym := by ext <;> rfl
 
-include wf₁ wf₂ in
 instance : (sym₁.mul sym₂).WF where
-  h_fs := by
-    simp [Raw.mul]; constructor
-    · have ⟨e₁, h₁, h₂⟩ := wf₁.h_fs.toBijectiveOn
-      have ⟨e₂, h₃, h₄⟩ := wf₂.h_fs.toBijectiveOn
-      use e₁.comp e₂; constructor <;> intro s hs <;> simp
-      rw [h₃ hs]; apply h₁; rw [h₂ hs]; apply h₄
-    · intro x h; apply wf₂.h_fs.cnd_of_right
-      exact wf₁.h_fs.cnd_of_right h
-    · intro x h; apply wf₁.h_fs.cnd_of_left
-      exact wf₂.h_fs.cnd_of_left h
-  h_ft := by
-    simp [Raw.mul]; constructor
-    · have ⟨e₁, h₁, h₂⟩ := wf₁.h_ft.toBijectiveOn
-      have ⟨e₂, h₃, h₄⟩ := wf₂.h_ft.toBijectiveOn
-      use e₁.comp e₂; constructor <;> intro s hs <;> simp
-      rw [h₃ hs]; apply h₁; rw [h₂ hs]; apply h₄
-    · intro x h; apply wf₂.h_ft.cnd_of_right
-      exact wf₁.h_ft.cnd_of_right h
-    · intro x h; apply wf₁.h_ft.cnd_of_left
-      exact wf₂.h_ft.cnd_of_left h
+  h_fs := by simp [mul]
+  h_fs' := by simp [mul]
+  h_ft := by simp [mul]
+  h_ft' := by simp [mul]
+  fs_fs' := by constructor <;> simp [mul]
+  ft_ft' := by constructor <;> simp [mul]
   tr_eq := by
-    intro s t hs; ext s'; simp [Raw.mul]; constructor
-    · intro h₁; have hs' := wf_of_tr h₁; use sym₁.fs # sym₂.fs s'
-      have ht := wfTrans_of_tr h₁; simp [tr_fs]; use s'
-    · rintro ⟨s', h₁, rfl⟩; have hs₁ := wf_of_tr h₁; simp [tr_ft] at h₁
-      obtain ⟨s', h₁, rfl⟩ := h₁; have hs' := wf_of_tr h₁; simpa
+    intro s t; ext s'; simp [mul]; constructor
+    · intro h₁; use sym₁.fs # sym₂.fs s'; simp [tr_fs]; use s'
+    · rintro ⟨s', h₁, rfl⟩; simp [tr_ft] at h₁; obtain ⟨s', h₁, rfl⟩ := h₁; simpa
   tr_eq' := by
-    intro s t hs; ext s'; simp [Raw.mul]; constructor
-    · intro h₁; have hs' := wf_of_tr h₁; use sym₂.fs' # sym₁.fs' s'
-      have ht := wfTrans_of_tr h₁; simp [tr_fs']; use s'
-    · rintro ⟨s', h₁, rfl⟩; have hs₁ := wf_of_tr h₁; simp [tr_ft'] at h₁
-      obtain ⟨s', h₁, rfl⟩ := h₁; have hs' := wf_of_tr h₁; simpa
+    intro s t; ext s'; simp [mul]; constructor
+    · intro h₁; use sym₂.fs' # sym₁.fs' s'; simp [tr_fs']; use s'
+    · rintro ⟨s', h₁, rfl⟩; simp [tr_ft'] at h₁; obtain ⟨s', h₁, rfl⟩ := h₁; simpa
 
-include wf in
+instance : (sym₁.div sym₂).WF := by
+  unfold div; infer_instance
+
 instance {n} : (sym.npow n).WF := by
-  simp [Raw.npow]; induction n; simp; infer_instance; nm n ih
+  simp [npow]; induction n; simp; infer_instance; nm n ih
   rw [Function.iterate_succ']; simp; infer_instance
 
-include wf in
 instance {z} : (sym.zpow z).WF := by
-  simp [Raw.zpow]; split <;> infer_instance
+  simp [zpow]; split <;> infer_instance
 
-structure Equiv (sym₁ sym₂ : Raw sys) : Prop where
-  hs : ∀ {s} [sys.WF s], sym₁.fs s = sym₂.fs s
-  hs' : ∀ {s} [sys.WF s], sym₁.fs' s = sym₂.fs' s
-  ht : ∀ {t} [sys.WFTrans t], sym₁.ft t = sym₂.ft t
-  ht' : ∀ {t} [sys.WFTrans t], sym₁.ft' t = sym₂.ft' t
+@[simp]
+protected theorem inv_mul_cancel : sym.inv.mul sym = one := by
+  simp [inv, mul, one]; constructor <;> ext <;> simp
 
-@[simp, refl]
-theorem Equiv.refl : sym.Equiv sym := by constructor <;> simp
-
-omit wf₁ wf₂ in @[symm]
-theorem Equiv.symm (h : sym₁.Equiv sym₂) : sym₂.Equiv sym₁ where
-  hs := h.hs.symm
-  hs' := h.hs'.symm
-  ht := h.ht.symm
-  ht' := h.ht'.symm
-
-omit wf₁ wf₂ wf₃ in @[trans]
-theorem Equiv.trans (h₁ : sym₁.Equiv sym₂) (h₂ : sym₂.Equiv sym₃) : sym₁.Equiv sym₃ where
-  hs := h₁.hs.trans # h₂.hs.trans # by rfl
-  hs' := h₁.hs'.trans # h₂.hs'.trans # by rfl
-  ht := h₁.ht.trans # h₂.ht.trans # by rfl
-  ht' := h₁.ht'.trans # h₂.ht'.trans # by rfl
-
-theorem Equiv.iseqv : Equivalence # Equiv (sys := sys) where
-  refl := λ _ => refl
-  symm := symm
-  trans := trans
-
-instance setoid : Setoid (Raw sys) where
-  r := Equiv
-  iseqv := Equiv.iseqv
+omit wf₁ @[simp]
+protected theorem inv_eq_of_mul (h : sym₁.mul sym₂ = one) : sym₁.inv = sym₂ := by
+  simp [inv, mul, one] at h ⊢; rcases h with ⟨h₁, h₂, h₃, h₄⟩; ext <;> dsimp
+  · nm s; apply congrArg sym₂.fs ∘ congrArg (· s) at h₂; simp at h₂; exact h₂
+  · nm s; apply congrArg (· # sym₂.fs' s) at h₁; simp at h₁; exact h₁
+  · nm t; apply congrArg sym₂.ft ∘ congrArg (· t) at h₄; simp at h₄; exact h₄
+  · nm t; apply congrArg (· # sym₂.ft' t) at h₃; simp at h₃; exact h₃
