AP/System/Symmetry/Basic.lean
@@ -1,3 +1,18 @@
 import AP.System.Symmetry.Defs
 
 namespace System.Symmetry
+
+universe u
+variable {S T : Type u} {sys : System S T}
+variable {sym sym₁ sym₂ sym₃ : Symmetry sys}
+
+instance : Group sys.Symmetry where
+  mul_assoc := λ _ _ _ => rfl
+  one_mul := λ _ => rfl
+  mul_one := λ _ => rfl
+  inv_mul_cancel := λ _ => ext Raw.inv_mul_cancel
+
+instance : DivisionMonoid sys.Symmetry where
+  mul_inv_rev := λ _ _ => rfl
+  inv_eq_of_mul := λ _ _ => by
+    simp only [Symmetry.ext_iff]; exact Raw.inv_eq_of_mul
